Fun.v
@@ -35,15 +35,7 @@ Lemma uni_upd A B (f g : A -> B) x fs :
   ~ indom fs x ->
   uni (update fs x tt) f g = upd (uni fs f g) x (f x).
 Proof.
-  move=>H; rewrite /update /upd/uni.
-  apply: functional_extensionality=>z.
-  have T: isTrue (x = z) -> x = z by apply istrue_isTrue_forw.
-  rewrite -!if_isTrue.
-  case:ifP=>H1; case:ifP=> H2; first by move:H2=>/T->.
-  Focus 2. (* I don't think this one is true *)
-Admitted.
-
-
+  (* move=> ?; extens=> d. *)
 Admitted.
 
 Lemma uni_nin A B (f g : A -> B) x fs : 
